core/RegSet.v
@@ -1,0 +1,15 @@
+From Stdlib Require Import ListSet.
+From Ssara.Core Require Import RegClass.
+
+Section RegSet.
+
+  Context {reg_instance : RegClass}.
+  
+  (* Set of virtual registers *)
+  Definition regs_union := set_union reg_eq_dec.
+  Definition regs_diff := set_diff reg_eq_dec.
+  Definition regs_add := set_add reg_eq_dec.
+  Definition regs_remove := set_remove reg_eq_dec.
+  Definition regs_mem := set_mem reg_eq_dec.
+
+End RegSet.
