core/Syntax.v
@@ -5,259 +5,259 @@ From Ssara.Core Require Import RegClass.
 
 Section Syntax.
 
-Context {reg_instance : RegClass}.
+  Context {reg_instance : RegClass}.
 
-Definition lbl := nat.
-Definition ptr := nat.
+  Definition lbl := nat.
+  Definition ptr := nat.
 
-(*
-  This represents a value that can either be an immediate number `x` or the
-  value contained in the register `r`
-*)
-Inductive val : Type :=
-  | Imm (x : Z)
-  | Reg (r : reg)
-  | Ptr (p : ptr)
-.
+  (*
+    This represents a value that can either be an immediate number `x` or the
+    value contained in the register `r`
+  *)
+  Inductive val : Type :=
+    | Imm (x : Z)
+    | Reg (r : reg)
+    | Ptr (p : ptr)
+  .
 
-Definition eq_val (v1 v2 : val) : bool :=
-  match v1, v2 with
-  | Imm x1, Imm x2 => Z.eqb x1 x2
-  | Reg x1, Reg x2 => reg_eqb x1 x2
-  | Ptr x1, Ptr x2 => Nat.eqb x1 x2
-  | _, _ => false
-  end
-.
-
-(*
-  The first operator of a binary expression is a `reg` because we assume that
-  an expression cannot have two constant arguments as the result can be
-  calculated in a previous stage of the compilation.
-  We avoided differentiating between unary, binary and n-ary expressions to
-  avoid having to deal with unnecessary nesting of data types.
-*)
-Inductive expr : Type :=
-  | Val : val -> expr
-  | Neg : val -> expr
-  | Load : val -> expr
-  | Add : reg -> val -> expr
-  | Sub : reg -> val -> expr
-  | Mul : reg -> val -> expr
-  | Div : reg -> val -> expr
-  | CmpLt : reg -> val -> expr
-  | CmpLe : reg -> val -> expr
-  | CmpGt : reg -> val -> expr
-  | CmpGe : reg -> val -> expr
-  | CmpEq : reg -> val -> expr
-  | CmpNe : reg -> val -> expr
-.
-
-Definition eq_expr (e1 e2 : expr) : bool :=
-  match e1, e2 with
-  | Val x1, Val x2 => eq_val x1 x2
-  | Neg x1, Neg x2 => eq_val x1 x2
-  | Load x1, Load x2 => eq_val x1 x2
-  | Add x1 y1, Add x2 y2 => (reg_eqb x1 x2) && (eq_val y1 y2)
-  | Sub x1 y1, Sub x2 y2 => (reg_eqb x1 x2) && (eq_val y1 y2)
-  | Mul x1 y1, Mul x2 y2 => (reg_eqb x1 x2) && (eq_val y1 y2)
-  | Div x1 y1, Div x2 y2 => (reg_eqb x1 x2) && (eq_val y1 y2)
-  | CmpLt x1 y1, CmpLt x2 y2 => (reg_eqb x1 x2) && (eq_val y1 y2)
-  | CmpLe x1 y1, CmpLe x2 y2 => (reg_eqb x1 x2) && (eq_val y1 y2)
-  | CmpGt x1 y1, CmpGt x2 y2 => (reg_eqb x1 x2) && (eq_val y1 y2)
-  | CmpGe x1 y1, CmpGe x2 y2 => (reg_eqb x1 x2) && (eq_val y1 y2)
-  | CmpEq x1 y1, CmpEq x2 y2 => (reg_eqb x1 x2) && (eq_val y1 y2)
-  | CmpNe x1 y1, CmpNe x2 y2 => (reg_eqb x1 x2) && (eq_val y1 y2)
-  | _, _ => false
-  end
-.
-
-Definition phi_arg : Type := (reg * lbl).
-
-(*
-  The `phi`, `inst` and `jinst` instructions are separated to avoid having to
-  deal with illegal basic blocks
-*)
-Inductive phi : Type :=
-  | Phi (r : reg) (rs: list phi_arg)
-.
-
-Definition phi_reg (p : phi) : reg :=
-  match p with
-  | Phi r _ => r
-  end
-.
-
-Definition phi_args (p : phi) : list phi_arg :=
-  match p with
-  | Phi _ rs => rs
-  end
-.
-
-Inductive inst : Type :=
-  | Def (r : reg) (e : expr)
-  | Swap (r : reg) (r' : reg)
-  | Store (v : val) (r : reg)
-.
-
-Definition inst_reg (i : inst) : list reg :=
-  match i with
-  | Def x _ => [x]
-  | Swap r r' => [r; r']
-  | Store _ _ => []
-  end
-.
-
-Definition inst_args (i : inst) : list reg :=
-  let reg_or_nil (v : val) : list reg :=
-    match v with
-    | Reg r => [r]
-    | _ => []
+  Definition eq_val (v1 v2 : val) : bool :=
+    match v1, v2 with
+    | Imm x1, Imm x2 => Z.eqb x1 x2
+    | Reg x1, Reg x2 => reg_eqb x1 x2
+    | Ptr x1, Ptr x2 => Nat.eqb x1 x2
+    | _, _ => false
     end
-  in
-  match i with
-  | Def x y =>
-    match y with
-    | Val v => reg_or_nil v
-    | Neg v => reg_or_nil v
-    | Load v => reg_or_nil v
-    | Add r v => r :: reg_or_nil v
-    | Sub r v => r :: reg_or_nil v
-    | Mul r v => r :: reg_or_nil v
-    | Div r v => r :: reg_or_nil v
-    | CmpLt r v => r :: reg_or_nil v
-    | CmpLe r v => r :: reg_or_nil v
-    | CmpGt r v => r :: reg_or_nil v
-    | CmpGe r v => r :: reg_or_nil v
-    | CmpEq r v => r :: reg_or_nil v
-    | CmpNe r v => r :: reg_or_nil v
+  .
+
+  (*
+    The first operator of a binary expression is a `reg` because we assume that
+    an expression cannot have two constant arguments as the result can be
+    calculated in a previous stage of the compilation.
+    We avoided differentiating between unary, binary and n-ary expressions to
+    avoid having to deal with unnecessary nesting of data types.
+  *)
+  Inductive expr : Type :=
+    | Val : val -> expr
+    | Neg : val -> expr
+    | Load : val -> expr
+    | Add : reg -> val -> expr
+    | Sub : reg -> val -> expr
+    | Mul : reg -> val -> expr
+    | Div : reg -> val -> expr
+    | CmpLt : reg -> val -> expr
+    | CmpLe : reg -> val -> expr
+    | CmpGt : reg -> val -> expr
+    | CmpGe : reg -> val -> expr
+    | CmpEq : reg -> val -> expr
+    | CmpNe : reg -> val -> expr
+  .
+
+  Definition eq_expr (e1 e2 : expr) : bool :=
+    match e1, e2 with
+    | Val x1, Val x2 => eq_val x1 x2
+    | Neg x1, Neg x2 => eq_val x1 x2
+    | Load x1, Load x2 => eq_val x1 x2
+    | Add x1 y1, Add x2 y2 => (reg_eqb x1 x2) && (eq_val y1 y2)
+    | Sub x1 y1, Sub x2 y2 => (reg_eqb x1 x2) && (eq_val y1 y2)
+    | Mul x1 y1, Mul x2 y2 => (reg_eqb x1 x2) && (eq_val y1 y2)
+    | Div x1 y1, Div x2 y2 => (reg_eqb x1 x2) && (eq_val y1 y2)
+    | CmpLt x1 y1, CmpLt x2 y2 => (reg_eqb x1 x2) && (eq_val y1 y2)
+    | CmpLe x1 y1, CmpLe x2 y2 => (reg_eqb x1 x2) && (eq_val y1 y2)
+    | CmpGt x1 y1, CmpGt x2 y2 => (reg_eqb x1 x2) && (eq_val y1 y2)
+    | CmpGe x1 y1, CmpGe x2 y2 => (reg_eqb x1 x2) && (eq_val y1 y2)
+    | CmpEq x1 y1, CmpEq x2 y2 => (reg_eqb x1 x2) && (eq_val y1 y2)
+    | CmpNe x1 y1, CmpNe x2 y2 => (reg_eqb x1 x2) && (eq_val y1 y2)
+    | _, _ => false
     end
-  | Swap r r' => r :: r' :: nil
-  | Store v r => r :: reg_or_nil v
-  end
-.
+  .
 
-(*
-  A block lbl is necessary in order to define the semantics of phi
-  instructions.
-*)
-CoInductive block : Type :=
-  | Block (l : lbl) (ps : list phi) (is : list inst) (j : jinst)
+  Definition phi_arg : Type := (reg * lbl).
 
-with jinst : Type :=
-  | Jnz (r : reg) (b1 : block) (b2 : block)
-  | Jmp (b : block)
-  | Halt
-.
+  (*
+    The `phi`, `inst` and `jinst` instructions are separated to avoid having to
+    deal with illegal basic blocks
+  *)
+  Inductive phi : Type :=
+    | Phi (r : reg) (rs: list phi_arg)
+  .
 
-Definition block_empty : block := Block O nil nil Halt.
-
-Definition jinst_args (j : jinst) : option reg :=
-  match j with
-  | Jnz r _ _ => Some r
-  | Jmp _ => None
-  | Halt => None
-  end
-.
-
-Definition get_lbl (b : block) : lbl :=
-  let (l, _, _, _) := b in l
-.
-
-Definition get_phis (b : block) : list phi :=
-  let (_, ps, _, _) := b in ps
-.
-
-Definition get_insts (b : block) : list inst :=
-  let (_, _, is, _) := b in is
-.
-
-Definition get_jinst (b : block) : jinst :=
-  let (_, _, _, j) := b in j
-.
-
-(*
-Fixpoint eq_jinst (j1 j2 : jinst) : bool :=
-  match j1, j2 with
-  | Jnz r b1 b2, Jnz r' b1' b2' => (Nat.eqb r r') && (eq_block b1 b1') && (eq_block b2 b2')
-  | Jmp b, Jmp b' => eq_block b b'
-  | Halt, Halt => true
-  | _, _ => false
-  end
-
-with eq_block (b1 : block) (b2 : block) : bool :=
-  match (b1, b2) with
-  | (Block ps1 is1 j1, Block ps2 is2 j2) =>
-    (eq_list_phi ps1 ps2)
-    && (eq_list_inst is1 is2)
-    && (eq_jinst j1 j2)
-  end
-.
-*)
-
-(* The starting block is the first block of CFG *)
-Definition program : Type := block.
-
-(*
-  Block instruction, represents all the possible instructions that could be
-  found inside a basic block
-*)
-Inductive binst : Type :=
-  | Bphi (p : phi)
-  | Binst (i : inst)
-  | Bjinst (j : jinst)
-.
-
-Definition start (p : program) : binst :=
-  let (_, ps, is, j) := p in
-  match ps with
-  | p :: _ => Bphi p
-  | nil =>
-    match is with
-    | i :: _ => Binst i
-    | nil => Bjinst j
+  Definition phi_reg (p : phi) : reg :=
+    match p with
+    | Phi r _ => r
     end
-  end
-.
+  .
 
-(*
-  ### Problems:
+  Definition phi_args (p : phi) : list phi_arg :=
+    match p with
+    | Phi _ rs => rs
+    end
+  .
 
-  - Allows reassigning the same register (enforced by the single_assignment_program predicate)
-  - Allows using unassigned registers (enforced by the assignment_dominates_usage predicate)
-  - Allows duplicate labels (solved by defining block recursivey)
-  - Allows jumping to unexistent labels (solved by defining block recursivey)
+  Inductive inst : Type :=
+    | Def (r : reg) (e : expr)
+    | Swap (r : reg) (r' : reg)
+    | Store (v : val) (r : reg)
+  .
 
-  We assume that all labels have a known destination
-  (there is no linking phase, or the linking already happened)
-  so we don't need to distinguish between internal jumps (known basic blocks)
-  and external jumps (unknown basic blocks that will be linked later)
-*)
+  Definition inst_reg (i : inst) : list reg :=
+    match i with
+    | Def x _ => [x]
+    | Swap r r' => [r; r']
+    | Store _ _ => []
+    end
+  .
 
-Definition successors (b : block) : list block :=
-  match get_jinst b with
-  | Jnz _ b1 b2 => [b1; b2]
-  | Jmp b => [b]
-  | Halt => []
-  end
-.
+  Definition inst_args (i : inst) : list reg :=
+    let reg_or_nil (v : val) : list reg :=
+      match v with
+      | Reg r => [r]
+      | _ => []
+      end
+    in
+    match i with
+    | Def x y =>
+      match y with
+      | Val v => reg_or_nil v
+      | Neg v => reg_or_nil v
+      | Load v => reg_or_nil v
+      | Add r v => r :: reg_or_nil v
+      | Sub r v => r :: reg_or_nil v
+      | Mul r v => r :: reg_or_nil v
+      | Div r v => r :: reg_or_nil v
+      | CmpLt r v => r :: reg_or_nil v
+      | CmpLe r v => r :: reg_or_nil v
+      | CmpGt r v => r :: reg_or_nil v
+      | CmpGe r v => r :: reg_or_nil v
+      | CmpEq r v => r :: reg_or_nil v
+      | CmpNe r v => r :: reg_or_nil v
+      end
+    | Swap r r' => r :: r' :: nil
+    | Store v r => r :: reg_or_nil v
+    end
+  .
 
-(*
-Definition predecessor (b : block) (b' : block) : bool :=
-  let (_, _, j) := b in
-  match j with
-  | Jnz _ b1 b2 => (eq_block b1 b') || (eq_block b2 b')
-  | Jmp b1 => eq_block b1 b'
-  | Halt => false
-  end
-.
+  (*
+    A block lbl is necessary in order to define the semantics of phi
+    instructions.
+  *)
+  CoInductive block : Type :=
+    | Block (l : lbl) (ps : list phi) (is : list inst) (j : jinst)
 
-Fixpoint predecessors (b : block) (p : program) : list block :=
-  match p with
-  | nil => nil
-  | b' :: bs => if predecessor b' b then b :: (predecessors b bs) else (predecessors b bs)
-  end
-.
-*)
+  with jinst : Type :=
+    | Jnz (r : reg) (b1 : block) (b2 : block)
+    | Jmp (b : block)
+    | Halt
+  .
+
+  Definition block_empty : block := Block O nil nil Halt.
+
+  Definition jinst_args (j : jinst) : option reg :=
+    match j with
+    | Jnz r _ _ => Some r
+    | Jmp _ => None
+    | Halt => None
+    end
+  .
+
+  Definition get_lbl (b : block) : lbl :=
+    let (l, _, _, _) := b in l
+  .
+
+  Definition get_phis (b : block) : list phi :=
+    let (_, ps, _, _) := b in ps
+  .
+
+  Definition get_insts (b : block) : list inst :=
+    let (_, _, is, _) := b in is
+  .
+
+  Definition get_jinst (b : block) : jinst :=
+    let (_, _, _, j) := b in j
+  .
+
+  (*
+  Fixpoint eq_jinst (j1 j2 : jinst) : bool :=
+    match j1, j2 with
+    | Jnz r b1 b2, Jnz r' b1' b2' => (Nat.eqb r r') && (eq_block b1 b1') && (eq_block b2 b2')
+    | Jmp b, Jmp b' => eq_block b b'
+    | Halt, Halt => true
+    | _, _ => false
+    end
+
+  with eq_block (b1 : block) (b2 : block) : bool :=
+    match (b1, b2) with
+    | (Block ps1 is1 j1, Block ps2 is2 j2) =>
+      (eq_list_phi ps1 ps2)
+      && (eq_list_inst is1 is2)
+      && (eq_jinst j1 j2)
+    end
+  .
+  *)
+
+  (* The starting block is the first block of CFG *)
+  Definition program : Type := block.
+
+  (*
+    Block instruction, represents all the possible instructions that could be
+    found inside a basic block
+  *)
+  Inductive binst : Type :=
+    | Bphi (p : phi)
+    | Binst (i : inst)
+    | Bjinst (j : jinst)
+  .
+
+  Definition start (p : program) : binst :=
+    let (_, ps, is, j) := p in
+    match ps with
+    | p :: _ => Bphi p
+    | nil =>
+      match is with
+      | i :: _ => Binst i
+      | nil => Bjinst j
+      end
+    end
+  .
+
+  (*
+    ### Problems:
+
+    - Allows reassigning the same register (enforced by the single_assignment_program predicate)
+    - Allows using unassigned registers (enforced by the assignment_dominates_usage predicate)
+    - Allows duplicate labels (solved by defining block recursivey)
+    - Allows jumping to unexistent labels (solved by defining block recursivey)
+
+    We assume that all labels have a known destination
+    (there is no linking phase, or the linking already happened)
+    so we don't need to distinguish between internal jumps (known basic blocks)
+    and external jumps (unknown basic blocks that will be linked later)
+  *)
+
+  Definition successors (b : block) : list block :=
+    match get_jinst b with
+    | Jnz _ b1 b2 => [b1; b2]
+    | Jmp b => [b]
+    | Halt => []
+    end
+  .
+
+  (*
+  Definition predecessor (b : block) (b' : block) : bool :=
+    let (_, _, j) := b in
+    match j with
+    | Jnz _ b1 b2 => (eq_block b1 b') || (eq_block b2 b')
+    | Jmp b1 => eq_block b1 b'
+    | Halt => false
+    end
+  .
+
+  Fixpoint predecessors (b : block) (p : program) : list block :=
+    match p with
+    | nil => nil
+    | b' :: bs => if predecessor b' b then b :: (predecessors b bs) else (predecessors b bs)
+    end
+  .
+  *)
 
 End Syntax.
 
