core/Utils.v
@@ -1,13 +1,3 @@
-From Ssara.Core Require Import Syntax.
-From Ssara.Core Require Import RegClass.
-From Ssara.Core Require Import Vm.
-From Stdlib Require Import ZArith.
-From Stdlib Require Import ListSet.
-From Stdlib Require Import Lists.List.
-
-From Ssara.Core Require Import RegVregInstance.
-Existing Instance reg_vreg_instance.
-
 (* Convert option to list *)
 Definition option_to_list {A : Type} (x : option A) : list A :=
   match x with
